<?xml version="1.0"?>
<rdf:RDF xmlns="http://purl.obolibrary.org/obo/psdo#"
     xml:base="http://purl.obolibrary.org/obo/psdo"
     xmlns:rdf="http://www.w3.org/1999/02/22-rdf-syntax-ns#"
     xmlns:owl="http://www.w3.org/2002/07/owl#"
     xmlns:oboInOwl="http://www.geneontology.org/formats/oboInOwl#"
     xmlns:xml="http://www.w3.org/XML/1998/namespace"
     xmlns:protege="http://protege.stanford.edu/plugins/owl/protege#"
     xmlns:xsd="http://www.w3.org/2001/XMLSchema#"
     xmlns:rdfs="http://www.w3.org/2000/01/rdf-schema#"
     xmlns:obo="http://purl.obolibrary.org/obo/"
     xmlns:foaf="http://xmlns.com/foaf/0.1/"
     xmlns:dc="http://purl.org/dc/elements/1.1/">
    <owl:Ontology rdf:about="http://purl.obolibrary.org/obo/psdo">
        <owl:imports rdf:resource="http://purl.obolibrary.org/obo/iao/2017-03-24/iao.owl"/>
        <owl:imports rdf:resource="http://purl.obolibrary.org/obo/ro/core.owl"/>
        <owl:imports rdf:resource="http://purl.obolibrary.org/obo/bfo/2.0/bfo.owl"/>
        <dc:license xml:lang="en">Ontology Content
The ontology content is licensed under a Creative Commons Attribution 4.0 International License.

Source Code
Copyright 2018 Regents of the University of Michigan

Licensed under the Apache License, Version 2.0 (the &quot;License&quot;);
you may not use this file except in compliance with the License.
You may obtain a copy of the License at

    http://www.apache.org/licenses/LICENSE-2.0

Unless required by applicable law or agreed to in writing, software
distributed under the License is distributed on an &quot;AS IS&quot; BASIS,
WITHOUT WARRANTIES OR CONDITIONS OF ANY KIND, either express or implied. See the License for the specific language governing permissions and limitations under the License.</dc:license>
        <dc:creator xml:lang="en">John Rincon</dc:creator>
        <dc:creator xml:lang="en">Cooper Stansbury</dc:creator>
        <owl:versionInfo xml:lang="en">1.0.0</owl:versionInfo>
        <dc:creator xml:lang="en">Zach Landis-Lewis</dc:creator>
        <dc:creator xml:lang="en">Colin Gross</dc:creator>
    </owl:Ontology>
    


    <!-- 
    ///////////////////////////////////////////////////////////////////////////////////////
    //
    // Classes
    //
    ///////////////////////////////////////////////////////////////////////////////////////
     -->

    


    <!-- http://purl.obolibrary.org/obo/psdo#psdo_0000001 -->

    <owl:Class rdf:about="http://purl.obolibrary.org/obo/psdo#psdo_0000001">
        <rdfs:subClassOf rdf:resource="http://purl.obolibrary.org/obo/IAO_0000030"/>
        <rdfs:subClassOf>
            <owl:Restriction>
                <owl:onProperty rdf:resource="http://purl.obolibrary.org/obo/BFO_0000051"/>
                <owl:someValuesFrom rdf:resource="http://purl.obolibrary.org/obo/psdo#psdo_0000008"/>
            </owl:Restriction>
        </rdfs:subClassOf>
        <rdfs:subClassOf>
            <owl:Restriction>
                <owl:onProperty rdf:resource="http://purl.obolibrary.org/obo/RO_0000058"/>
                <owl:someValuesFrom rdf:resource="http://purl.obolibrary.org/obo/psdo#psdo_0000079"/>
            </owl:Restriction>
        </rdfs:subClassOf>
        <obo:IAO_0000115 xml:lang="en">An information content entity that displays relations between dimensions in a concretized collection of display components.</obo:IAO_0000115>
        <obo:IAO_0000119 xml:lang="en">Zhang J. A representational analysis of relational information displays. International Journal of Human-Computer Studies. 1996 Jul 1;45(1):59–74.</obo:IAO_0000119>
        <obo:IAO_0000232 xml:lang="en">Zhang’s notion of &apos;dimension&apos; relies on an understanding of ‘distributed representations’ which have both an &apos;internal&apos; and an &apos;external&apos; component. Each dimension (see &apos;representing dimension&apos;) has a quality of &apos;being distrobuted between internal (the cognition and representation of the dimension as such) and external (the &apos;mark).&apos; See:

Zhang J, Norman DA. Representations in distributed cognitive tasks. Cognitive Science. 1994 Jan 1;18(1):87–122.</obo:IAO_0000232>
        <rdfs:label xml:lang="en">relational information display</rdfs:label>
    </owl:Class>
    


    <!-- http://purl.obolibrary.org/obo/psdo#psdo_0000002 -->

    <owl:Class rdf:about="http://purl.obolibrary.org/obo/psdo#psdo_0000002">
        <rdfs:subClassOf rdf:resource="http://purl.obolibrary.org/obo/IAO_0000030"/>
        <obo:IAO_0000115 xml:lang="en">An information content entity that is the collection of specification and metadata associated with a generalized potential information display.</obo:IAO_0000115>
        <rdfs:label xml:lang="en">performance summary display template</rdfs:label>
    </owl:Class>
    


    <!-- http://purl.obolibrary.org/obo/psdo#psdo_0000003 -->

    <owl:Class rdf:about="http://purl.obolibrary.org/obo/psdo#psdo_0000003">
        <rdfs:subClassOf rdf:resource="http://purl.obolibrary.org/obo/psdo#psdo_0000001"/>
        <rdfs:subClassOf>
            <owl:Restriction>
                <owl:onProperty rdf:resource="http://purl.obolibrary.org/obo/IAO_0000136"/>
                <owl:someValuesFrom rdf:resource="http://purl.obolibrary.org/obo/psdo#psdo_0000006"/>
            </owl:Restriction>
        </rdfs:subClassOf>
        <obo:IAO_0000115 xml:lang="en">A relational information display whose display components bear some combination of dimension roles: ascribee dimension, performance measure dimension, performance dimension, or time dimension.</obo:IAO_0000115>
        <obo:IAO_0000117>Cooper Stansbury, John Rincon, Dahee Lee, Zach Landis-Lewis, Colin Gross</obo:IAO_0000117>
        <obo:IAO_0000232 xml:lang="en">All subclasses of &apos;performance summary display&apos; are defined classes based on cardinality of marks that realize specific represented dimension roles.</obo:IAO_0000232>
        <obo:IAO_0000232 xml:lang="en">It is the authors current belief that the necessary and sufficient definiton of &apos;performance summary display&apos; mandates that at least two dimensions must be realized.</obo:IAO_0000232>
        <rdfs:label xml:lang="en">performance summary display</rdfs:label>
    </owl:Class>
    


    <!-- http://purl.obolibrary.org/obo/psdo#psdo_0000004 -->

    <owl:Class rdf:about="http://purl.obolibrary.org/obo/psdo#psdo_0000004">
        <rdfs:subClassOf rdf:resource="http://purl.obolibrary.org/obo/psdo#psdo_0000042"/>
        <obo:IAO_0000115>A data item that is a statement about the recorded output of measurements, aggregates, and/or calculations, or decisions related to measured behavior</obo:IAO_0000115>
        <rdfs:label rdf:datatype="http://www.w3.org/2001/XMLSchema#string">obsolete performance data</rdfs:label>
        <owl:deprecated rdf:datatype="http://www.w3.org/2001/XMLSchema#boolean">true</owl:deprecated>
    </owl:Class>
    


    <!-- http://purl.obolibrary.org/obo/psdo#psdo_0000006 -->

    <owl:Class rdf:about="http://purl.obolibrary.org/obo/psdo#psdo_0000006">
        <rdfs:subClassOf rdf:resource="http://purl.obolibrary.org/obo/BFO_0000023"/>
        <rdfs:subClassOf>
            <owl:Class>
                <owl:unionOf rdf:parseType="Collection">
                    <owl:Restriction>
                        <owl:onProperty rdf:resource="http://purl.obolibrary.org/obo/RO_0000052"/>
                        <owl:someValuesFrom rdf:resource="http://purl.obolibrary.org/obo/psdo#psdo_0000062"/>
                    </owl:Restriction>
                    <owl:Restriction>
                        <owl:onProperty rdf:resource="http://purl.obolibrary.org/obo/RO_0000052"/>
                        <owl:someValuesFrom rdf:resource="http://purl.obolibrary.org/obo/psdo#psdo_0000079"/>
                    </owl:Restriction>
                </owl:unionOf>
            </owl:Class>
        </rdfs:subClassOf>
        <obo:IAO_0000115 xml:lang="en">A role inhering in the set of attributes of a mark that share a scale type and that convey information about something in a relational information display.</obo:IAO_0000115>
        <obo:IAO_0000119 xml:lang="en">Zhang J. A representational analysis of relational information displays. International Journal of Human-Computer Studies. 1996 Jul 1;45(1):59–74.</obo:IAO_0000119>
        <obo:IAO_0000232 xml:lang="en">&apos;Represented dimensions&apos; are realized in the processes perception, design or cognition.</obo:IAO_0000232>
        <rdfs:label xml:lang="en">represented dimension</rdfs:label>
    </owl:Class>
    


    <!-- http://purl.obolibrary.org/obo/psdo#psdo_0000008 -->

    <owl:Class rdf:about="http://purl.obolibrary.org/obo/psdo#psdo_0000008">
        <rdfs:subClassOf rdf:resource="http://purl.obolibrary.org/obo/IAO_0000030"/>
        <rdfs:subClassOf>
            <owl:Restriction>
                <owl:onProperty rdf:resource="http://purl.obolibrary.org/obo/BFO_0000050"/>
                <owl:someValuesFrom rdf:resource="http://purl.obolibrary.org/obo/psdo#psdo_0000001"/>
            </owl:Restriction>
        </rdfs:subClassOf>
        <obo:IAO_0000112>An axis, a title of an axis or of a graph, a bar in a bar graph, a line in a line graph, a textual entity in a table.</obo:IAO_0000112>
        <obo:IAO_0000115 xml:lang="en">An information content entity that is a proper part of a relational information display and is concretized by a mark.</obo:IAO_0000115>
        <obo:IAO_0000232 xml:lang="en">Munzner T. Visualization analysis and design. Boca Raton: CRC Press, Taylor &amp; Francis Group, CRC Press is an imprint of the Taylor &amp; Francis Group, an informa business; 2015. 404 p. (A.K. Peters visualization series).</obo:IAO_0000232>
        <obo:IAO_0000232 xml:lang="en">The material entity that concretizes the information content entity has the capability to bear some role &apos;represented dimension&apos; or &apos;focal element, ect...</obo:IAO_0000232>
        <rdfs:label xml:lang="en">relational information display component</rdfs:label>
    </owl:Class>
    


    <!-- http://purl.obolibrary.org/obo/psdo#psdo_0000017 -->

    <owl:Class rdf:about="http://purl.obolibrary.org/obo/psdo#psdo_0000017">
        <rdfs:subClassOf rdf:resource="http://purl.obolibrary.org/obo/psdo#psdo_0000042"/>
        <obo:IAO_0000115 xml:lang="en">the property of a space in a dataset or relational information display that indicates that &apos;n&apos; mutually perpendicular linear directions of movement are possible</obo:IAO_0000115>
        <obo:IAO_0000116 xml:lang="en">Formally, saying a &quot;space&quot; has n dimensions means that you can find n vectors in the &quot;space&quot; for which none is a linear combination of the others. In addition, in any set of n + 1 vectors one of them can be written as a linear combination of the other n vectors</obo:IAO_0000116>
        <obo:IAO_0000116 xml:lang="en">each dimension is a set of elements (di1, di2, di3 ... din) from 1. Zhang J. A representational analysis of relational information displays. International Journal of Human-Computer Studies. 1996 Jul 1;45(1):59–74.</obo:IAO_0000116>
        <obo:IAO_0000119 xml:lang="en">1. Mathwords: Dimensions [Internet]. [cited 2018 Jun 8]. Available from: http://www.mathwords.com/d/dimensions.htm</obo:IAO_0000119>
        <rdfs:label rdf:datatype="http://www.w3.org/2001/XMLSchema#string">obsolete dimension</rdfs:label>
        <owl:deprecated rdf:datatype="http://www.w3.org/2001/XMLSchema#boolean">true</owl:deprecated>
    </owl:Class>
    


    <!-- http://purl.obolibrary.org/obo/psdo#psdo_0000018 -->

    <owl:Class rdf:about="http://purl.obolibrary.org/obo/psdo#psdo_0000018">
        <rdfs:subClassOf rdf:resource="http://purl.obolibrary.org/obo/psdo#psdo_0000006"/>
        <obo:IAO_0000115 xml:lang="en">A represented dimension where the attributes of the mark are about entities that have attributed performance data.</obo:IAO_0000115>
        <obo:IAO_0000232 xml:lang="en">The elements of an &apos;ascribee dimension&apos; typically represent people, organizations, or groups. They can also represent statistics, targets, or goals. The possible overlap with &apos;performance measure dimension&apos; is justified by the creative liberties taken by the designer of the performance summary display.</obo:IAO_0000232>
        <rdfs:label xml:lang="en">ascribee dimension</rdfs:label>
    </owl:Class>
    


    <!-- http://purl.obolibrary.org/obo/psdo#psdo_0000019 -->

    <owl:Class rdf:about="http://purl.obolibrary.org/obo/psdo#psdo_0000019">
        <rdfs:subClassOf rdf:resource="http://purl.obolibrary.org/obo/BFO_0000023"/>
        <rdfs:subClassOf>
            <owl:Class>
                <owl:unionOf rdf:parseType="Collection">
                    <owl:Restriction>
                        <owl:onProperty rdf:resource="http://purl.obolibrary.org/obo/RO_0000052"/>
                        <owl:someValuesFrom rdf:resource="http://purl.obolibrary.org/obo/psdo#psdo_0000062"/>
                    </owl:Restriction>
                    <owl:Restriction>
                        <owl:onProperty rdf:resource="http://purl.obolibrary.org/obo/RO_0000052"/>
                        <owl:someValuesFrom rdf:resource="http://purl.obolibrary.org/obo/psdo#psdo_0000079"/>
                    </owl:Restriction>
                </owl:unionOf>
            </owl:Class>
        </rdfs:subClassOf>
        <obo:IAO_0000115 xml:lang="en">A role inhering in a mark that is disjoint with a focal element and that has the same scale type as the focal element.</obo:IAO_0000115>
        <rdfs:label xml:lang="en">comparative element</rdfs:label>
    </owl:Class>
    


    <!-- http://purl.obolibrary.org/obo/psdo#psdo_0000020 -->

    <owl:Class rdf:about="http://purl.obolibrary.org/obo/psdo#psdo_0000020">
        <rdfs:subClassOf rdf:resource="http://purl.obolibrary.org/obo/BFO_0000019"/>
        <rdfs:subClassOf>
            <owl:Restriction>
                <owl:onProperty rdf:resource="http://purl.obolibrary.org/obo/RO_0000080"/>
                <owl:someValuesFrom rdf:resource="http://purl.obolibrary.org/obo/psdo#psdo_0000062"/>
            </owl:Restriction>
        </rdfs:subClassOf>
        <obo:IAO_0000115 xml:lang="en">A quality that is the abstract measurement property of a concretized display component.</obo:IAO_0000115>
        <obo:IAO_0000119 xml:lang="en">Zhang J. A representational analysis of relational information displays. International Journal of Human-Computer Studies. 1996 Jul 1;45(1):59–74.</obo:IAO_0000119>
        <rdfs:label xml:lang="en">scale type</rdfs:label>
    </owl:Class>
    


    <!-- http://purl.obolibrary.org/obo/psdo#psdo_0000021 -->

    <owl:Class rdf:about="http://purl.obolibrary.org/obo/psdo#psdo_0000021">
        <rdfs:subClassOf rdf:resource="http://purl.obolibrary.org/obo/psdo#psdo_0000042"/>
        <obo:IAO_0000115>a scale type without equal interval or absolute zero properties</obo:IAO_0000115>
        <obo:IAO_0000116>def circular and needs work</obo:IAO_0000116>
        <rdfs:label rdf:datatype="http://www.w3.org/2001/XMLSchema#string">obsolete discrete scale types</rdfs:label>
        <owl:deprecated rdf:datatype="http://www.w3.org/2001/XMLSchema#boolean">true</owl:deprecated>
    </owl:Class>
    


    <!-- http://purl.obolibrary.org/obo/psdo#psdo_0000022 -->

    <owl:Class rdf:about="http://purl.obolibrary.org/obo/psdo#psdo_0000022">
        <rdfs:subClassOf rdf:resource="http://purl.obolibrary.org/obo/psdo#psdo_0000042"/>
        <obo:IAO_0000115>a scale type that be measured in infinitely small units</obo:IAO_0000115>
        <obo:IAO_0000116>def circular and needs work</obo:IAO_0000116>
        <rdfs:label rdf:datatype="http://www.w3.org/2001/XMLSchema#string">obsolete continuous scale types</rdfs:label>
        <owl:deprecated rdf:datatype="http://www.w3.org/2001/XMLSchema#boolean">true</owl:deprecated>
    </owl:Class>
    


    <!-- http://purl.obolibrary.org/obo/psdo#psdo_0000023 -->

    <owl:Class rdf:about="http://purl.obolibrary.org/obo/psdo#psdo_0000023">
        <rdfs:subClassOf rdf:resource="http://purl.obolibrary.org/obo/psdo#psdo_0000020"/>
        <rdfs:subClassOf>
            <owl:Restriction>
                <owl:onProperty rdf:resource="http://purl.obolibrary.org/obo/RO_0000080"/>
                <owl:someValuesFrom rdf:resource="http://purl.obolibrary.org/obo/psdo#psdo_0000062"/>
            </owl:Restriction>
        </rdfs:subClassOf>
        <obo:IAO_0000115 xml:lang="en">A scale type with three formal properties that (1) the instances can be distinguished from each other and (2) that one instance on a scale can be judged greater than, less than, or equal to another instance on the same scale and that (3) the magnitude of an instance represented by a unit on the scale is the same regardless of where on the scale the unit falls.</obo:IAO_0000115>
        <obo:IAO_0000119 xml:lang="en">Zhang J. A representational analysis of relational information displays. International Journal of Human-Computer Studies. 1996 Jul 1;45(1):59–74.</obo:IAO_0000119>
        <rdfs:label xml:lang="en">interval scale</rdfs:label>
    </owl:Class>
    


    <!-- http://purl.obolibrary.org/obo/psdo#psdo_0000024 -->

    <owl:Class rdf:about="http://purl.obolibrary.org/obo/psdo#psdo_0000024">
        <rdfs:subClassOf rdf:resource="http://purl.obolibrary.org/obo/psdo#psdo_0000020"/>
        <rdfs:subClassOf>
            <owl:Restriction>
                <owl:onProperty rdf:resource="http://purl.obolibrary.org/obo/RO_0000080"/>
                <owl:someValuesFrom rdf:resource="http://purl.obolibrary.org/obo/psdo#psdo_0000062"/>
            </owl:Restriction>
        </rdfs:subClassOf>
        <obo:IAO_0000115 xml:lang="en">A scale type with four formal properties that (1) the instances can be distinguished from each other and (2) that one instance on a scale can be judged greater than, less than, or equal to another instance on the same scale, that (3) the magnitude of an instance represented by a unit on the scale is the same regardless of where on the scale the unit falls and (4) an absolute zero value can indicate that nothing at all of the property being represented exists.</obo:IAO_0000115>
        <obo:IAO_0000119 xml:lang="en">Zhang J. A representational analysis of relational information displays. International Journal of Human-Computer Studies. 1996 Jul 1;45(1):59–74.</obo:IAO_0000119>
        <rdfs:label xml:lang="en">ratio scale</rdfs:label>
    </owl:Class>
    


    <!-- http://purl.obolibrary.org/obo/psdo#psdo_0000025 -->

    <owl:Class rdf:about="http://purl.obolibrary.org/obo/psdo#psdo_0000025">
        <rdfs:subClassOf rdf:resource="http://purl.obolibrary.org/obo/psdo#psdo_0000020"/>
        <rdfs:subClassOf>
            <owl:Restriction>
                <owl:onProperty rdf:resource="http://purl.obolibrary.org/obo/RO_0000080"/>
                <owl:someValuesFrom rdf:resource="http://purl.obolibrary.org/obo/psdo#psdo_0000062"/>
            </owl:Restriction>
        </rdfs:subClassOf>
        <obo:IAO_0000115 xml:lang="en">A scale type with two formal properties that (1) the instances can be distinguished from each other and (2) that one instance on a scale can be judged greater than, less than, or equal to another instance on the same scale.</obo:IAO_0000115>
        <obo:IAO_0000119 xml:lang="en">Zhang J. A representational analysis of relational information displays. International Journal of Human-Computer Studies. 1996 Jul 1;45(1):59–74.</obo:IAO_0000119>
        <rdfs:label xml:lang="en">ordinal scale</rdfs:label>
    </owl:Class>
    


    <!-- http://purl.obolibrary.org/obo/psdo#psdo_0000026 -->

    <owl:Class rdf:about="http://purl.obolibrary.org/obo/psdo#psdo_0000026">
        <rdfs:subClassOf rdf:resource="http://purl.obolibrary.org/obo/psdo#psdo_0000020"/>
        <rdfs:subClassOf>
            <owl:Restriction>
                <owl:onProperty rdf:resource="http://purl.obolibrary.org/obo/RO_0000080"/>
                <owl:someValuesFrom rdf:resource="http://purl.obolibrary.org/obo/psdo#psdo_0000062"/>
            </owl:Restriction>
        </rdfs:subClassOf>
        <obo:IAO_0000115 xml:lang="en">A scale type with one  formal property that (1) the instances can be distinguished from each other.</obo:IAO_0000115>
        <obo:IAO_0000119 xml:lang="en">Zhang J. A representational analysis of relational information displays. International Journal of Human-Computer Studies. 1996 Jul 1;45(1):59–74.</obo:IAO_0000119>
        <rdfs:label xml:lang="en">nominal scale</rdfs:label>
    </owl:Class>
    


    <!-- http://purl.obolibrary.org/obo/psdo#psdo_0000027 -->

    <owl:Class rdf:about="http://purl.obolibrary.org/obo/psdo#psdo_0000027">
        <rdfs:subClassOf rdf:resource="http://purl.obolibrary.org/obo/psdo#psdo_0000042"/>
        <rdfs:label rdf:datatype="http://www.w3.org/2001/XMLSchema#string">obsolete time series</rdfs:label>
        <owl:deprecated rdf:datatype="http://www.w3.org/2001/XMLSchema#boolean">true</owl:deprecated>
    </owl:Class>
    


    <!-- http://purl.obolibrary.org/obo/psdo#psdo_0000028 -->

    <owl:Class rdf:about="http://purl.obolibrary.org/obo/psdo#psdo_0000028">
        <rdfs:subClassOf rdf:resource="http://purl.obolibrary.org/obo/BFO_0000145"/>
        <obo:IAO_0000115 xml:lang="en">A relational quality of the perceived general movement of a mark, or set of marks that is integrated over a time dimension.</obo:IAO_0000115>
        <rdfs:label xml:lang="en">performance trend</rdfs:label>
    </owl:Class>
    


    <!-- http://purl.obolibrary.org/obo/psdo#psdo_0000029 -->

    <owl:Class rdf:about="http://purl.obolibrary.org/obo/psdo#psdo_0000029">
        <rdfs:subClassOf rdf:resource="http://purl.obolibrary.org/obo/BFO_0000145"/>
        <obo:IAO_0000115 xml:lang="en">A relational quality of the perceived distance between marks.</obo:IAO_0000115>
        <rdfs:label xml:lang="en">performance gap</rdfs:label>
    </owl:Class>
    


    <!-- http://purl.obolibrary.org/obo/psdo#psdo_0000031 -->

    <owl:Class rdf:about="http://purl.obolibrary.org/obo/psdo#psdo_0000031">
        <rdfs:subClassOf rdf:resource="http://purl.obolibrary.org/obo/IAO_0000088"/>
        <obo:IAO_0000115 xml:lang="en">A report designed for the purpose of providing performance summary information to a recipient of an intervention.</obo:IAO_0000115>
        <rdfs:label xml:lang="en">performance report</rdfs:label>
    </owl:Class>
    


    <!-- http://purl.obolibrary.org/obo/psdo#psdo_0000035 -->

    <owl:Class rdf:about="http://purl.obolibrary.org/obo/psdo#psdo_0000035">
        <rdfs:subClassOf rdf:resource="http://purl.obolibrary.org/obo/psdo#psdo_0000006"/>
        <obo:IAO_0000112 xml:lang="en">Two sepearate performance measure elements might be &apos;appropriate perscriptions of Drug A&apos; and &apos;appropriate perscriptions of Drug B.&apos; Each performance has a method for measurement that is specific to the type of drug (A or B) prescription behavior.</obo:IAO_0000112>
        <obo:IAO_0000115 xml:lang="en">A represented dimension where the attributes of the mark are about the methods of measuring behavior.</obo:IAO_0000115>
        <rdfs:label xml:lang="en">performance measure dimension</rdfs:label>
    </owl:Class>
    


    <!-- http://purl.obolibrary.org/obo/psdo#psdo_0000036 -->

    <owl:Class rdf:about="http://purl.obolibrary.org/obo/psdo#psdo_0000036">
        <rdfs:subClassOf rdf:resource="http://purl.obolibrary.org/obo/psdo#psdo_0000006"/>
        <obo:IAO_0000115 xml:lang="en">A represented dimension where the attributes of the mark are about time.</obo:IAO_0000115>
        <rdfs:label xml:lang="en">time dimension</rdfs:label>
    </owl:Class>
    


    <!-- http://purl.obolibrary.org/obo/psdo#psdo_0000037 -->

    <owl:Class rdf:about="http://purl.obolibrary.org/obo/psdo#psdo_0000037">
        <rdfs:subClassOf rdf:resource="http://purl.obolibrary.org/obo/psdo#psdo_0000006"/>
        <obo:IAO_0000115 xml:lang="en">A represented dimension where the attributes of the mark are about measurements, decisions, aggregates, or calculations related to measured behavior.</obo:IAO_0000115>
        <obo:IAO_0000232 xml:lang="en">Performance dimension can include entities like performance values (all scale types)</obo:IAO_0000232>
        <rdfs:label xml:lang="en">performance dimension</rdfs:label>
    </owl:Class>
    


    <!-- http://purl.obolibrary.org/obo/psdo#psdo_0000040 -->

    <owl:Class rdf:about="http://purl.obolibrary.org/obo/psdo#psdo_0000040">
        <rdfs:subClassOf rdf:resource="http://purl.obolibrary.org/obo/BFO_0000023"/>
        <rdfs:subClassOf>
            <owl:Restriction>
                <owl:onProperty rdf:resource="http://purl.obolibrary.org/obo/RO_0000052"/>
                <owl:someValuesFrom rdf:resource="http://purl.obolibrary.org/obo/psdo#psdo_0000062"/>
            </owl:Restriction>
        </rdfs:subClassOf>
        <obo:IAO_0000115 xml:lang="en">A role inhering in a mark that conveys specific information to the recipient of a performance summary report realized through the acts of perception.</obo:IAO_0000115>
        <rdfs:label xml:lang="en">focal element</rdfs:label>
    </owl:Class>
    


    <!-- http://purl.obolibrary.org/obo/psdo#psdo_0000041 -->

    <owl:Class rdf:about="http://purl.obolibrary.org/obo/psdo#psdo_0000041">
        <rdfs:subClassOf rdf:resource="http://purl.obolibrary.org/obo/psdo#psdo_0000040"/>
        <obo:IAO_0000115 xml:lang="en">A focal element that conveys information about identity to the recipient of the performance summary report.</obo:IAO_0000115>
        <rdfs:label xml:lang="en">recipient element</rdfs:label>
    </owl:Class>
    


    <!-- http://purl.obolibrary.org/obo/psdo#psdo_0000042 -->

    <owl:Class rdf:about="http://purl.obolibrary.org/obo/psdo#psdo_0000042">
        <rdfs:subClassOf rdf:resource="http://www.geneontology.org/formats/oboInOwl#ObsoleteClass"/>
        <rdfs:label rdf:datatype="http://www.w3.org/2001/XMLSchema#string">obsolete obsolete class</rdfs:label>
        <owl:deprecated rdf:datatype="http://www.w3.org/2001/XMLSchema#boolean">true</owl:deprecated>
    </owl:Class>
    


    <!-- http://purl.obolibrary.org/obo/psdo#psdo_0000043 -->

    <owl:Class rdf:about="http://purl.obolibrary.org/obo/psdo#psdo_0000043">
        <rdfs:subClassOf rdf:resource="http://purl.obolibrary.org/obo/psdo#psdo_0000042"/>
        <obo:IAO_0000115>the perception of emergent properties between dimensions, or elements of dimension of relational information displays</obo:IAO_0000115>
        <rdfs:label rdf:datatype="http://www.w3.org/2001/XMLSchema#string">obsolete relational perceptions</rdfs:label>
        <owl:deprecated rdf:datatype="http://www.w3.org/2001/XMLSchema#boolean">true</owl:deprecated>
    </owl:Class>
    


    <!-- http://purl.obolibrary.org/obo/psdo#psdo_0000045 -->

    <owl:Class rdf:about="http://purl.obolibrary.org/obo/psdo#psdo_0000045">
        <rdfs:subClassOf rdf:resource="http://purl.obolibrary.org/obo/psdo#psdo_0000019"/>
        <obo:IAO_0000115 xml:lang="en">A comparative element that conveys information about an entity that has an attributed performance value.</obo:IAO_0000115>
        <rdfs:label xml:lang="en">social comparator</rdfs:label>
    </owl:Class>
    


    <!-- http://purl.obolibrary.org/obo/psdo#psdo_0000046 -->

    <owl:Class rdf:about="http://purl.obolibrary.org/obo/psdo#psdo_0000046">
        <rdfs:subClassOf rdf:resource="http://purl.obolibrary.org/obo/psdo#psdo_0000019"/>
        <obo:IAO_0000115 xml:lang="en">A comparative element that conveys information about a desired future performance value.</obo:IAO_0000115>
        <rdfs:label xml:lang="en">goal comparator</rdfs:label>
    </owl:Class>
    


    <!-- http://purl.obolibrary.org/obo/psdo#psdo_0000047 -->

    <owl:Class rdf:about="http://purl.obolibrary.org/obo/psdo#psdo_0000047">
        <rdfs:subClassOf rdf:resource="http://purl.obolibrary.org/obo/psdo#psdo_0000019"/>
        <obo:IAO_0000115 xml:lang="en">A comparative element that conveys information about a predetermined performance value.</obo:IAO_0000115>
        <rdfs:label xml:lang="en">standard comparator</rdfs:label>
    </owl:Class>
    


    <!-- http://purl.obolibrary.org/obo/psdo#psdo_0000048 -->

    <owl:Class rdf:about="http://purl.obolibrary.org/obo/psdo#psdo_0000048">
        <rdfs:subClassOf rdf:resource="http://purl.obolibrary.org/obo/psdo#psdo_0000042"/>
        <obo:IAO_0000112>the textual entity: &apos;John E. Doe&apos; is a perfomer data item.</obo:IAO_0000112>
        <obo:IAO_0000115>A data item that is a statement about entities which can have attributed performance data</obo:IAO_0000115>
        <rdfs:label rdf:datatype="http://www.w3.org/2001/XMLSchema#string">obsolete performer data</rdfs:label>
        <owl:deprecated rdf:datatype="http://www.w3.org/2001/XMLSchema#boolean">true</owl:deprecated>
    </owl:Class>
    


    <!-- http://purl.obolibrary.org/obo/psdo#psdo_0000049 -->

    <owl:Class rdf:about="http://purl.obolibrary.org/obo/psdo#psdo_0000049">
        <rdfs:subClassOf rdf:resource="http://purl.obolibrary.org/obo/psdo#psdo_0000042"/>
        <obo:IAO_0000115>A data item that is a statement about time</obo:IAO_0000115>
        <rdfs:label rdf:datatype="http://www.w3.org/2001/XMLSchema#string">obsolete time data</rdfs:label>
        <owl:deprecated rdf:datatype="http://www.w3.org/2001/XMLSchema#boolean">true</owl:deprecated>
    </owl:Class>
    


    <!-- http://purl.obolibrary.org/obo/psdo#psdo_0000050 -->

    <owl:Class rdf:about="http://purl.obolibrary.org/obo/psdo#psdo_0000050">
        <rdfs:subClassOf rdf:resource="http://purl.obolibrary.org/obo/psdo#psdo_0000042"/>
        <obo:IAO_0000112>the textual entity: &apos;appropriate prescription of drug A&apos; is a performance measurement data item that is about the method of collecting data for the behavior &apos;prescribing drug A.&apos;  The result of this method is a performance data item.</obo:IAO_0000112>
        <obo:IAO_0000115>a data item that is a statement about a method of measuring performance data</obo:IAO_0000115>
        <rdfs:label rdf:datatype="http://www.w3.org/2001/XMLSchema#string">obsolete performance measurement data</rdfs:label>
        <owl:deprecated rdf:datatype="http://www.w3.org/2001/XMLSchema#boolean">true</owl:deprecated>
    </owl:Class>
    


    <!-- http://purl.obolibrary.org/obo/psdo#psdo_0000053 -->

    <owl:Class rdf:about="http://purl.obolibrary.org/obo/psdo#psdo_0000053">
        <rdfs:subClassOf rdf:resource="http://purl.obolibrary.org/obo/psdo#psdo_0000042"/>
        <rdfs:label rdf:datatype="http://www.w3.org/2001/XMLSchema#string">obsolete mark</rdfs:label>
        <owl:deprecated rdf:datatype="http://www.w3.org/2001/XMLSchema#boolean">true</owl:deprecated>
    </owl:Class>
    


    <!-- http://purl.obolibrary.org/obo/psdo#psdo_0000054 -->

    <owl:Class rdf:about="http://purl.obolibrary.org/obo/psdo#psdo_0000054">
        <rdfs:subClassOf rdf:resource="http://purl.obolibrary.org/obo/psdo#psdo_0000061"/>
        <obo:IAO_0000115 xml:lang="en">An attribute of external form or contour.</obo:IAO_0000115>
        <obo:IAO_0000119 xml:lang="en">&quot;shape, n.1.&quot; OED Online, Oxford University Press, June 2018, www.oed.com/view/Entry/177498. Accessed 28 June 2018.</obo:IAO_0000119>
        <rdfs:label xml:lang="en">shape</rdfs:label>
    </owl:Class>
    


    <!-- http://purl.obolibrary.org/obo/psdo#psdo_0000055 -->

    <owl:Class rdf:about="http://purl.obolibrary.org/obo/psdo#psdo_0000055">
        <rdfs:subClassOf rdf:resource="http://purl.obolibrary.org/obo/psdo#psdo_0000061"/>
        <obo:IAO_0000115 xml:lang="en">An attribute by virtue of which some thing appears to have a color.</obo:IAO_0000115>
        <obo:IAO_0000119 xml:lang="en">&quot;colour | color, n.1.&quot; OED Online, Oxford University Press, June 2018, www.oed.com/view/Entry/36596. Accessed 28 June 2018.</obo:IAO_0000119>
        <rdfs:label xml:lang="en">color</rdfs:label>
    </owl:Class>
    


    <!-- http://purl.obolibrary.org/obo/psdo#psdo_0000056 -->

    <owl:Class rdf:about="http://purl.obolibrary.org/obo/psdo#psdo_0000056">
        <rdfs:subClassOf rdf:resource="http://purl.obolibrary.org/obo/psdo#psdo_0000061"/>
        <obo:IAO_0000115 xml:lang="en">An attribute of relation in which a thing stands with respect to another or others.</obo:IAO_0000115>
        <obo:IAO_0000119 xml:lang="en">&quot;position, n.&quot; OED Online, Oxford University Press, June 2018, www.oed.com/view/Entry/148314. Accessed 28 June 2018.</obo:IAO_0000119>
        <obo:IAO_0000232>&apos;Position’ may actually be a relational quality in BFO because is depends on multiple entities.</obo:IAO_0000232>
        <rdfs:label xml:lang="en">position</rdfs:label>
    </owl:Class>
    


    <!-- http://purl.obolibrary.org/obo/psdo#psdo_0000057 -->

    <owl:Class rdf:about="http://purl.obolibrary.org/obo/psdo#psdo_0000057">
        <rdfs:subClassOf rdf:resource="http://www.geneontology.org/formats/oboInOwl#ObsoleteClass"/>
        <obo:IAO_0000115 xml:lang="en">def needed</obo:IAO_0000115>
        <rdfs:label rdf:datatype="http://www.w3.org/2001/XMLSchema#string">obsolete text</rdfs:label>
        <owl:deprecated rdf:datatype="http://www.w3.org/2001/XMLSchema#boolean">true</owl:deprecated>
    </owl:Class>
    


    <!-- http://purl.obolibrary.org/obo/psdo#psdo_0000058 -->

    <owl:Class rdf:about="http://purl.obolibrary.org/obo/psdo#psdo_0000058">
        <rdfs:subClassOf rdf:resource="http://purl.obolibrary.org/obo/psdo#psdo_0000061"/>
        <obo:IAO_0000115 xml:lang="en">An attribute of the magnitude of the degree of divergence of two things from one another.</obo:IAO_0000115>
        <obo:IAO_0000119 xml:lang="en">&quot;angle, n.2.&quot; OED Online, Oxford University Press, June 2018, www.oed.com/view/Entry/7542. Accessed 28 June 2018.</obo:IAO_0000119>
        <obo:IAO_0000232>&apos;Angle’ may actually be a relational quality in BFO because is depends on multiple entities.</obo:IAO_0000232>
        <rdfs:label xml:lang="en">angle</rdfs:label>
    </owl:Class>
    


    <!-- http://purl.obolibrary.org/obo/psdo#psdo_0000059 -->

    <owl:Class rdf:about="http://purl.obolibrary.org/obo/psdo#psdo_0000059">
        <rdfs:subClassOf rdf:resource="http://purl.obolibrary.org/obo/psdo#psdo_0000061"/>
        <obo:IAO_0000115 xml:lang="en">An attribute of constitution, structure, or substance of anything with regard to its constituents or formative element.</obo:IAO_0000115>
        <obo:IAO_0000119 xml:lang="en">&quot;texture, n.&quot; OED Online, Oxford University Press, June 2018, www.oed.com/view/Entry/200031. Accessed 28 June 2018.</obo:IAO_0000119>
        <rdfs:label xml:lang="en">texture</rdfs:label>
    </owl:Class>
    


    <!-- http://purl.obolibrary.org/obo/psdo#psdo_0000060 -->

    <owl:Class rdf:about="http://purl.obolibrary.org/obo/psdo#psdo_0000060">
        <rdfs:subClassOf rdf:resource="http://purl.obolibrary.org/obo/psdo#psdo_0000061"/>
        <obo:IAO_0000115 xml:lang="en">the quality of linear magnitude of any thing as measured from end to end</obo:IAO_0000115>
        <obo:IAO_0000119 xml:lang="en">&quot;length, n.&quot; OED Online, Oxford University Press, June 2018, www.oed.com/view/Entry/107245. Accessed 28 June 2018.</obo:IAO_0000119>
        <obo:IAO_0000232 xml:lang="en">rdfs:Label property is &apos;mark length&apos; to distinguish from the PATO class &apos;length.&apos;</obo:IAO_0000232>
        <rdfs:label xml:lang="en">mark length</rdfs:label>
    </owl:Class>
    


    <!-- http://purl.obolibrary.org/obo/psdo#psdo_0000061 -->

    <owl:Class rdf:about="http://purl.obolibrary.org/obo/psdo#psdo_0000061">
        <rdfs:subClassOf rdf:resource="http://purl.obolibrary.org/obo/IAO_0000015"/>
        <rdfs:subClassOf>
            <owl:Restriction>
                <owl:onProperty rdf:resource="http://purl.obolibrary.org/obo/RO_0000080"/>
                <owl:someValuesFrom rdf:resource="http://purl.obolibrary.org/obo/psdo#psdo_0000062"/>
            </owl:Restriction>
        </rdfs:subClassOf>
        <obo:IAO_0000115 xml:lang="en">An information carrier that can be measured, observed, or logged.</obo:IAO_0000115>
        <obo:IAO_0000119 xml:lang="en">Munzner T. Visualization analysis and design. Boca Raton: CRC Press, Taylor &amp; Francis Group, CRC Press is an imprint of the Taylor &amp; Francis Group, an informa business; 2015. 404 p. (A.K. Peters visualization series).</obo:IAO_0000119>
        <rdfs:label xml:lang="en">attribute</rdfs:label>
    </owl:Class>
    


    <!-- http://purl.obolibrary.org/obo/psdo#psdo_0000062 -->

    <owl:Class rdf:about="http://purl.obolibrary.org/obo/psdo#psdo_0000062">
        <owl:equivalentClass>
            <owl:Class>
                <owl:intersectionOf rdf:parseType="Collection">
                    <rdf:Description rdf:about="http://purl.obolibrary.org/obo/IAO_0000178"/>
                    <owl:Restriction>
                        <owl:onProperty rdf:resource="http://purl.obolibrary.org/obo/RO_0000053"/>
                        <owl:someValuesFrom>
                            <owl:Restriction>
                                <owl:onProperty rdf:resource="http://purl.obolibrary.org/obo/RO_0000059"/>
                                <owl:someValuesFrom rdf:resource="http://purl.obolibrary.org/obo/psdo#psdo_0000008"/>
                            </owl:Restriction>
                        </owl:someValuesFrom>
                    </owl:Restriction>
                </owl:intersectionOf>
            </owl:Class>
        </owl:equivalentClass>
        <rdfs:subClassOf rdf:resource="http://purl.obolibrary.org/obo/IAO_0000178"/>
        <obo:IAO_0000112 xml:lang="en">Ink on paper or pixels on a screen (non-exhaustive).</obo:IAO_0000112>
        <obo:IAO_0000115 xml:lang="en">A material information bearer that is a basic visual element of a relational information display.</obo:IAO_0000115>
        <obo:IAO_0000119 xml:lang="en">Munzner T. Visualization analysis and design. Boca Raton: CRC Press, Taylor &amp; Francis Group, CRC Press is an imprint of the Taylor &amp; Francis Group, an informa business; 2015. 404 p. (A.K. Peters visualization series).</obo:IAO_0000119>
        <rdfs:label xml:lang="en">mark</rdfs:label>
    </owl:Class>
    


    <!-- http://purl.obolibrary.org/obo/psdo#psdo_0000065 -->

    <owl:Class rdf:about="http://purl.obolibrary.org/obo/psdo#psdo_0000065">
        <rdfs:subClassOf rdf:resource="http://purl.obolibrary.org/obo/psdo#psdo_0000003"/>
        <obo:IAO_0000115 xml:lang="en">**WARNING** This is a placeholder class whose IRI will be used to query different PSDOs with different dimensional cardinalities (as defined classes). The semantic label and defintion will be changed to reflect different subclasses of PSDO once that taxonomy is formalized.</obo:IAO_0000115>
        <rdfs:label xml:lang="en">label TDB</rdfs:label>
    </owl:Class>
    


    <!-- http://purl.obolibrary.org/obo/psdo#psdo_0000066 -->

    <owl:Class rdf:about="http://purl.obolibrary.org/obo/psdo#psdo_0000066">
        <rdfs:subClassOf rdf:resource="http://purl.obolibrary.org/obo/psdo#psdo_0000003"/>
        <obo:IAO_0000115 xml:lang="en">**WARNING** This is a placeholder class whose IRI will be used to query different PSDOs with different dimensional cardinalities (as defined classes). The semantic label and defintion will be changed to reflect different subclasses of PSDO once that taxonomy is formalized.</obo:IAO_0000115>
        <rdfs:label xml:lang="en">label TDB</rdfs:label>
    </owl:Class>
    


    <!-- http://purl.obolibrary.org/obo/psdo#psdo_0000067 -->

    <owl:Class rdf:about="http://purl.obolibrary.org/obo/psdo#psdo_0000067">
        <rdfs:subClassOf rdf:resource="http://purl.obolibrary.org/obo/psdo#psdo_0000065"/>
        <obo:IAO_0000115 xml:lang="en">**WARNING** This is a placeholder class whose IRI will be used to query different PSDOs with different dimensional cardinalities (as defined classes). The semantic label and defintion will be changed to reflect different subclasses of PSDO once that taxonomy is formalized.</obo:IAO_0000115>
        <rdfs:label xml:lang="en">label TDB</rdfs:label>
    </owl:Class>
    


    <!-- http://purl.obolibrary.org/obo/psdo#psdo_0000068 -->

    <owl:Class rdf:about="http://purl.obolibrary.org/obo/psdo#psdo_0000068">
        <rdfs:subClassOf rdf:resource="http://purl.obolibrary.org/obo/psdo#psdo_0000065"/>
        <obo:IAO_0000115 xml:lang="en">**WARNING** This is a placeholder class whose IRI will be used to query different PSDOs with different dimensional cardinalities (as defined classes). The semantic label and defintion will be changed to reflect different subclasses of PSDO once that taxonomy is formalized.</obo:IAO_0000115>
        <rdfs:label xml:lang="en">label TDB</rdfs:label>
    </owl:Class>
    


    <!-- http://purl.obolibrary.org/obo/psdo#psdo_0000069 -->

    <owl:Class rdf:about="http://purl.obolibrary.org/obo/psdo#psdo_0000069">
        <rdfs:subClassOf rdf:resource="http://purl.obolibrary.org/obo/psdo#psdo_0000066"/>
        <obo:IAO_0000115 xml:lang="en">**WARNING** This is a placeholder class whose IRI will be used to query different PSDOs with different dimensional cardinalities (as defined classes). The semantic label and defintion will be changed to reflect different subclasses of PSDO once that taxonomy is formalized.</obo:IAO_0000115>
        <rdfs:label xml:lang="en">label TDB</rdfs:label>
    </owl:Class>
    


    <!-- http://purl.obolibrary.org/obo/psdo#psdo_0000070 -->

    <owl:Class rdf:about="http://purl.obolibrary.org/obo/psdo#psdo_0000070">
        <rdfs:subClassOf rdf:resource="http://purl.obolibrary.org/obo/psdo#psdo_0000066"/>
        <obo:IAO_0000115 xml:lang="en">**WARNING** This is a placeholder class whose IRI will be used to query different PSDOs with different dimensional cardinalities (as defined classes). The semantic label and defintion will be changed to reflect different subclasses of PSDO once that taxonomy is formalized.</obo:IAO_0000115>
        <rdfs:label xml:lang="en">label TDB</rdfs:label>
    </owl:Class>
    


    <!-- http://purl.obolibrary.org/obo/psdo#psdo_0000071 -->

    <owl:Class rdf:about="http://purl.obolibrary.org/obo/psdo#psdo_0000071">
        <rdfs:subClassOf rdf:resource="http://purl.obolibrary.org/obo/psdo#psdo_0000070"/>
        <obo:IAO_0000115 xml:lang="en">**WARNING** This is a placeholder class whose IRI will be used to query different PSDOs with different dimensional cardinalities (as defined classes). The semantic label and defintion will be changed to reflect different subclasses of PSDO once that taxonomy is formalized.</obo:IAO_0000115>
        <rdfs:label xml:lang="en">label TDB</rdfs:label>
    </owl:Class>
    


    <!-- http://purl.obolibrary.org/obo/psdo#psdo_0000072 -->

    <owl:Class rdf:about="http://purl.obolibrary.org/obo/psdo#psdo_0000072">
        <rdfs:subClassOf rdf:resource="http://purl.obolibrary.org/obo/psdo#psdo_0000070"/>
        <obo:IAO_0000115 xml:lang="en">**WARNING** This is a placeholder class whose IRI will be used to query different PSDOs with different dimensional cardinalities (as defined classes). The semantic label and defintion will be changed to reflect different subclasses of PSDO once that taxonomy is formalized.</obo:IAO_0000115>
        <rdfs:label xml:lang="en">label TDB</rdfs:label>
    </owl:Class>
    


    <!-- http://purl.obolibrary.org/obo/psdo#psdo_0000073 -->

    <owl:Class rdf:about="http://purl.obolibrary.org/obo/psdo#psdo_0000073">
        <rdfs:subClassOf rdf:resource="http://purl.obolibrary.org/obo/psdo#psdo_0000069"/>
        <obo:IAO_0000115 xml:lang="en">**WARNING** This is a placeholder class whose IRI will be used to query different PSDOs with different dimensional cardinalities (as defined classes). The semantic label and defintion will be changed to reflect different subclasses of PSDO once that taxonomy is formalized.</obo:IAO_0000115>
        <rdfs:label xml:lang="en">label TDB</rdfs:label>
    </owl:Class>
    


    <!-- http://purl.obolibrary.org/obo/psdo#psdo_0000074 -->

    <owl:Class rdf:about="http://purl.obolibrary.org/obo/psdo#psdo_0000074">
        <rdfs:subClassOf rdf:resource="http://purl.obolibrary.org/obo/psdo#psdo_0000069"/>
        <obo:IAO_0000115 xml:lang="en">**WARNING** This is a placeholder class whose IRI will be used to query different PSDOs with different dimensional cardinalities (as defined classes). The semantic label and defintion will be changed to reflect different subclasses of PSDO once that taxonomy is formalized.</obo:IAO_0000115>
        <rdfs:label xml:lang="en">label TDB</rdfs:label>
    </owl:Class>
    


    <!-- http://purl.obolibrary.org/obo/psdo#psdo_0000075 -->

    <owl:Class rdf:about="http://purl.obolibrary.org/obo/psdo#psdo_0000075">
        <rdfs:subClassOf rdf:resource="http://purl.obolibrary.org/obo/psdo#psdo_0000068"/>
        <obo:IAO_0000115 xml:lang="en">**WARNING** This is a placeholder class whose IRI will be used to query different PSDOs with different dimensional cardinalities (as defined classes). The semantic label and defintion will be changed to reflect different subclasses of PSDO once that taxonomy is formalized.</obo:IAO_0000115>
        <rdfs:label xml:lang="en">label TDB</rdfs:label>
    </owl:Class>
    


    <!-- http://purl.obolibrary.org/obo/psdo#psdo_0000076 -->

    <owl:Class rdf:about="http://purl.obolibrary.org/obo/psdo#psdo_0000076">
        <rdfs:subClassOf rdf:resource="http://purl.obolibrary.org/obo/psdo#psdo_0000068"/>
        <obo:IAO_0000115 xml:lang="en">**WARNING** This is a placeholder class whose IRI will be used to query different PSDOs with different dimensional cardinalities (as defined classes). The semantic label and defintion will be changed to reflect different subclasses of PSDO once that taxonomy is formalized.</obo:IAO_0000115>
        <rdfs:label xml:lang="en">label TDB</rdfs:label>
    </owl:Class>
    


    <!-- http://purl.obolibrary.org/obo/psdo#psdo_0000077 -->

    <owl:Class rdf:about="http://purl.obolibrary.org/obo/psdo#psdo_0000077">
        <rdfs:subClassOf rdf:resource="http://purl.obolibrary.org/obo/psdo#psdo_0000067"/>
        <obo:IAO_0000115 xml:lang="en">**WARNING** This is a placeholder class whose IRI will be used to query different PSDOs with different dimensional cardinalities (as defined classes). The semantic label and defintion will be changed to reflect different subclasses of PSDO once that taxonomy is formalized.</obo:IAO_0000115>
        <rdfs:label xml:lang="en">label TDB</rdfs:label>
    </owl:Class>
    


    <!-- http://purl.obolibrary.org/obo/psdo#psdo_0000078 -->

    <owl:Class rdf:about="http://purl.obolibrary.org/obo/psdo#psdo_0000078">
        <rdfs:subClassOf rdf:resource="http://purl.obolibrary.org/obo/psdo#psdo_0000067"/>
        <obo:IAO_0000115 xml:lang="en">**WARNING** This is a placeholder class whose IRI will be used to query different PSDOs with different dimensional cardinalities (as defined classes). The semantic label and defintion will be changed to reflect different subclasses of PSDO once that taxonomy is formalized.</obo:IAO_0000115>
        <rdfs:label xml:lang="en">label TDB</rdfs:label>
    </owl:Class>
    


    <!-- http://purl.obolibrary.org/obo/psdo#psdo_0000079 -->

    <owl:Class rdf:about="http://purl.obolibrary.org/obo/psdo#psdo_0000079">
        <rdfs:subClassOf rdf:resource="http://purl.obolibrary.org/obo/BFO_0000027"/>
        <rdfs:subClassOf>
            <owl:Restriction>
                <owl:onProperty rdf:resource="http://purl.obolibrary.org/obo/RO_0002351"/>
                <owl:someValuesFrom rdf:resource="http://purl.obolibrary.org/obo/psdo#psdo_0000062"/>
            </owl:Restriction>
        </rdfs:subClassOf>
        <obo:IAO_0000115 xml:lang="en">A object aggregate of marks.</obo:IAO_0000115>
        <rdfs:label xml:lang="en">mark collection</rdfs:label>
    </owl:Class>
</rdf:RDF>



<!-- Generated by the OWL API (version 4.2.8.20170104-2310) https://github.com/owlcs/owlapi -->

