<?xml version="1.0"?>
<rdf:RDF xmlns="http://purl.obolibrary.org/obo/psdo#"
     xml:base="http://purl.obolibrary.org/obo/psdo"
     xmlns:rdf="http://www.w3.org/1999/02/22-rdf-syntax-ns#"
     xmlns:owl="http://www.w3.org/2002/07/owl#"
     xmlns:xml="http://www.w3.org/XML/1998/namespace"
     xmlns:xsd="http://www.w3.org/2001/XMLSchema#"
     xmlns:rdfs="http://www.w3.org/2000/01/rdf-schema#"
     xmlns:obo="http://purl.obolibrary.org/obo/"
     xmlns:foaf="http://xmlns.com/foaf/0.1/"
     xmlns:dc="http://purl.org/dc/elements/1.1/">
    <owl:Ontology rdf:about="http://purl.obolibrary.org/obo/psdo">
        <owl:imports rdf:resource="http://purl.obolibrary.org/obo/iao-slim.owl"/>
        <owl:imports rdf:resource="http://purl.obolibrary.org/obo/bfo/2.0/bfo.owl"/>
        <dc:contributor>Cooper Stansbury</dc:contributor>
        <dc:contributor>John Rincon</dc:contributor>
        <owl:versionInfo>0.0.2</owl:versionInfo>
        <dc:contributor>Colin Gross</dc:contributor>
        <obo:IAO_0000232>Based loosley on an analysis of the following works:

1. Zhang J. A representational analysis of relational information displays. International Journal of Human-Computer Studies. 1996 Jul 1;45(1):59–74.</obo:IAO_0000232>
        <dc:contributor>Zach Landis-Lewis</dc:contributor>
        <dc:license>Need to insert license</dc:license>
    </owl:Ontology>
    


    <!-- 
    ///////////////////////////////////////////////////////////////////////////////////////
    //
    // Classes
    //
    ///////////////////////////////////////////////////////////////////////////////////////
     -->

    


    <!-- http://purl.obolibrary.org/obo/IAO_0000027 -->

    <rdf:Description rdf:about="http://purl.obolibrary.org/obo/IAO_0000027">
        <rdfs:subClassOf rdf:resource="http://purl.obolibrary.org/obo/IAO_0000030"/>
    </rdf:Description>
    


    <!-- http://purl.obolibrary.org/obo/IAO_0000030 -->

    <rdf:Description rdf:about="http://purl.obolibrary.org/obo/IAO_0000030">
        <rdfs:subClassOf rdf:resource="http://purl.obolibrary.org/obo/BFO_0000031"/>
    </rdf:Description>
    


    <!-- http://purl.obolibrary.org/obo/IAO_0000088 -->

    <rdf:Description rdf:about="http://purl.obolibrary.org/obo/IAO_0000088">
        <rdfs:subClassOf rdf:resource="http://purl.obolibrary.org/obo/IAO_0000310"/>
    </rdf:Description>
    


    <!-- http://purl.obolibrary.org/obo/IAO_0000100 -->

    <rdf:Description rdf:about="http://purl.obolibrary.org/obo/IAO_0000100">
        <rdfs:subClassOf rdf:resource="http://purl.obolibrary.org/obo/IAO_0000030"/>
    </rdf:Description>
    


    <!-- http://purl.obolibrary.org/obo/IAO_0000109 -->

    <rdf:Description rdf:about="http://purl.obolibrary.org/obo/IAO_0000109">
        <rdfs:subClassOf rdf:resource="http://purl.obolibrary.org/obo/IAO_0000027"/>
    </rdf:Description>
    


    <!-- http://purl.obolibrary.org/obo/IAO_0000310 -->

    <rdf:Description rdf:about="http://purl.obolibrary.org/obo/IAO_0000310">
        <rdfs:subClassOf rdf:resource="http://purl.obolibrary.org/obo/IAO_0000030"/>
    </rdf:Description>
    


    <!-- http://purl.obolibrary.org/obo/psdo#psdo_0000001 -->

    <owl:Class rdf:about="http://purl.obolibrary.org/obo/psdo#psdo_0000001">
        <rdfs:subClassOf rdf:resource="http://purl.obolibrary.org/obo/IAO_0000030"/>
        <obo:IAO_0000115>A display which represents relations between dimensions.</obo:IAO_0000115>
        <obo:IAO_0000119>1. Zhang J. A representational analysis of relational information displays. International Journal of Human-Computer Studies. 1996 Jul 1;45(1):59–74.</obo:IAO_0000119>
        <rdfs:label xml:lang="en">relational information display</rdfs:label>
    </owl:Class>
    


    <!-- http://purl.obolibrary.org/obo/psdo#psdo_0000002 -->

    <owl:Class rdf:about="http://purl.obolibrary.org/obo/psdo#psdo_0000002">
        <rdfs:subClassOf rdf:resource="http://purl.obolibrary.org/obo/IAO_0000030"/>
        <obo:IAO_0000115>the specifications and metadata associated with a relational information display</obo:IAO_0000115>
        <rdfs:label xml:lang="en">relational information display template</rdfs:label>
    </owl:Class>
    


    <!-- http://purl.obolibrary.org/obo/psdo#psdo_0000003 -->

    <owl:Class rdf:about="http://purl.obolibrary.org/obo/psdo#psdo_0000003">
        <rdfs:subClassOf rdf:resource="http://purl.obolibrary.org/obo/psdo#psdo_0000001"/>
        <rdfs:comment>A relational information display that represents dimensions of performer, performance measure, performance data, and time.</rdfs:comment>
        <rdfs:label xml:lang="en">performance summary display</rdfs:label>
    </owl:Class>
    


    <!-- http://purl.obolibrary.org/obo/psdo#psdo_0000004 -->

    <owl:Class rdf:about="http://purl.obolibrary.org/obo/psdo#psdo_0000004">
        <rdfs:subClassOf rdf:resource="http://purl.obolibrary.org/obo/IAO_0000027"/>
        <obo:IAO_0000115>A documented outcome of the targeted behavior that results from processes such as performance measurement, prediction, or goal-setting.</obo:IAO_0000115>
        <rdfs:label xml:lang="en">performance data</rdfs:label>
    </owl:Class>
    


    <!-- http://purl.obolibrary.org/obo/psdo#psdo_0000005 -->

    <owl:Class rdf:about="http://purl.obolibrary.org/obo/psdo#psdo_0000005">
        <rdfs:subClassOf rdf:resource="http://purl.obolibrary.org/obo/BFO_0000019"/>
        <obo:IAO_0000115>the number of &apos;n&apos; mutually perpendicular directions of motion that are possible</obo:IAO_0000115>
        <rdfs:label xml:lang="en">dimsension cardinality</rdfs:label>
    </owl:Class>
    


    <!-- http://purl.obolibrary.org/obo/psdo#psdo_0000006 -->

    <owl:Class rdf:about="http://purl.obolibrary.org/obo/psdo#psdo_0000006">
        <rdfs:subClassOf rdf:resource="http://purl.obolibrary.org/obo/psdo#psdo_0000017"/>
        <obo:IAO_0000119>a dimensional space that represents something in reality, i.e., is realized in a physical bearer that is a graphical or numeric component of a relational information display or a dataset</obo:IAO_0000119>
        <rdfs:label xml:lang="en">represented dimension</rdfs:label>
    </owl:Class>
    


    <!-- http://purl.obolibrary.org/obo/psdo#psdo_0000007 -->

    <owl:Class rdf:about="http://purl.obolibrary.org/obo/psdo#psdo_0000007">
        <rdfs:subClassOf rdf:resource="http://purl.obolibrary.org/obo/psdo#psdo_0000003"/>
        <rdfs:label xml:lang="en">performance graph</rdfs:label>
    </owl:Class>
    


    <!-- http://purl.obolibrary.org/obo/psdo#psdo_0000008 -->

    <owl:Class rdf:about="http://purl.obolibrary.org/obo/psdo#psdo_0000008">
        <rdfs:subClassOf rdf:resource="http://purl.obolibrary.org/obo/IAO_0000030"/>
        <obo:IAO_0000115>modular components of a relational information display, i.e., the physical &quot;objects&quot; that are concretized that can be &quot;related&quot;</obo:IAO_0000115>
        <rdfs:label xml:lang="en">physical graphical component</rdfs:label>
    </owl:Class>
    


    <!-- http://purl.obolibrary.org/obo/psdo#psdo_0000009 -->

    <owl:Class rdf:about="http://purl.obolibrary.org/obo/psdo#psdo_0000009">
        <rdfs:subClassOf rdf:resource="http://purl.obolibrary.org/obo/psdo#psdo_0000008"/>
        <rdfs:label xml:lang="en">bar</rdfs:label>
    </owl:Class>
    


    <!-- http://purl.obolibrary.org/obo/psdo#psdo_0000010 -->

    <owl:Class rdf:about="http://purl.obolibrary.org/obo/psdo#psdo_0000010">
        <rdfs:subClassOf rdf:resource="http://purl.obolibrary.org/obo/psdo#psdo_0000008"/>
        <rdfs:label xml:lang="en">line</rdfs:label>
    </owl:Class>
    


    <!-- http://purl.obolibrary.org/obo/psdo#psdo_0000011 -->

    <owl:Class rdf:about="http://purl.obolibrary.org/obo/psdo#psdo_0000011">
        <rdfs:subClassOf rdf:resource="http://purl.obolibrary.org/obo/psdo#psdo_0000008"/>
        <rdfs:label xml:lang="en">dot</rdfs:label>
    </owl:Class>
    


    <!-- http://purl.obolibrary.org/obo/psdo#psdo_0000012 -->

    <owl:Class rdf:about="http://purl.obolibrary.org/obo/psdo#psdo_0000012">
        <rdfs:subClassOf rdf:resource="http://purl.obolibrary.org/obo/psdo#psdo_0000003"/>
        <rdfs:label xml:lang="en">performance table</rdfs:label>
    </owl:Class>
    


    <!-- http://purl.obolibrary.org/obo/psdo#psdo_0000013 -->

    <owl:Class rdf:about="http://purl.obolibrary.org/obo/psdo#psdo_0000013">
        <rdfs:subClassOf rdf:resource="http://purl.obolibrary.org/obo/psdo#psdo_0000008"/>
        <rdfs:label xml:lang="en">legend</rdfs:label>
    </owl:Class>
    


    <!-- http://purl.obolibrary.org/obo/psdo#psdo_0000014 -->

    <owl:Class rdf:about="http://purl.obolibrary.org/obo/psdo#psdo_0000014">
        <rdfs:subClassOf rdf:resource="http://purl.obolibrary.org/obo/psdo#psdo_0000008"/>
        <rdfs:label xml:lang="en">label</rdfs:label>
    </owl:Class>
    


    <!-- http://purl.obolibrary.org/obo/psdo#psdo_0000015 -->

    <owl:Class rdf:about="http://purl.obolibrary.org/obo/psdo#psdo_0000015">
        <rdfs:subClassOf rdf:resource="http://purl.obolibrary.org/obo/psdo#psdo_0000008"/>
        <rdfs:label xml:lang="en">axis</rdfs:label>
    </owl:Class>
    


    <!-- http://purl.obolibrary.org/obo/psdo#psdo_0000016 -->

    <owl:Class rdf:about="http://purl.obolibrary.org/obo/psdo#psdo_0000016">
        <rdfs:subClassOf rdf:resource="http://purl.obolibrary.org/obo/psdo#psdo_0000008"/>
        <rdfs:label xml:lang="en">text</rdfs:label>
    </owl:Class>
    


    <!-- http://purl.obolibrary.org/obo/psdo#psdo_0000017 -->

    <owl:Class rdf:about="http://purl.obolibrary.org/obo/psdo#psdo_0000017">
        <rdfs:subClassOf rdf:resource="http://purl.obolibrary.org/obo/BFO_0000023"/>
        <obo:IAO_0000115>the property of a space in a dataset or relational information display that indicates that n mutually perpendicular linear directions of movement are possible</obo:IAO_0000115>
        <obo:IAO_0000116>Formally, saying a &quot;space&quot; has n dimensions means that you can find n vectors in the &quot;space&quot; for which none is a linear combination of the others. In addition, in any set of n + 1 vectors one of them can be written as a linear combination of the other n vectors</obo:IAO_0000116>
        <obo:IAO_0000116>each dimension is a set of elements (di1, di2, di3 ... din) from 1. Zhang J. A representational analysis of relational information displays. International Journal of Human-Computer Studies. 1996 Jul 1;45(1):59–74.</obo:IAO_0000116>
        <obo:IAO_0000119>1. Mathwords: Dimensions [Internet]. [cited 2018 Jun 8]. Available from: http://www.mathwords.com/d/dimensions.htm</obo:IAO_0000119>
        <rdfs:label xml:lang="en">dimension</rdfs:label>
    </owl:Class>
    


    <!-- http://purl.obolibrary.org/obo/psdo#psdo_0000018 -->

    <owl:Class rdf:about="http://purl.obolibrary.org/obo/psdo#psdo_0000018">
        <rdfs:subClassOf rdf:resource="http://purl.obolibrary.org/obo/psdo#psdo_0000006"/>
        <obo:IAO_0000115>a vector that represents people, organizations, or other agents that engage in measured behavior(s)</obo:IAO_0000115>
        <rdfs:label xml:lang="en">performer dimension</rdfs:label>
    </owl:Class>
    


    <!-- http://purl.obolibrary.org/obo/psdo#psdo_0000019 -->

    <owl:Class rdf:about="http://purl.obolibrary.org/obo/psdo#psdo_0000019">
        <rdfs:label xml:lang="en">comparator</rdfs:label>
    </owl:Class>
    


    <!-- http://purl.obolibrary.org/obo/psdo#psdo_0000020 -->

    <owl:Class rdf:about="http://purl.obolibrary.org/obo/psdo#psdo_0000020">
        <rdfs:subClassOf rdf:resource="http://purl.obolibrary.org/obo/BFO_0000019"/>
        <rdfs:label xml:lang="en">scale type</rdfs:label>
    </owl:Class>
    


    <!-- http://purl.obolibrary.org/obo/psdo#psdo_0000021 -->

    <owl:Class rdf:about="http://purl.obolibrary.org/obo/psdo#psdo_0000021">
        <rdfs:subClassOf rdf:resource="http://purl.obolibrary.org/obo/psdo#psdo_0000020"/>
        <rdfs:label xml:lang="en">discrete scale types</rdfs:label>
    </owl:Class>
    


    <!-- http://purl.obolibrary.org/obo/psdo#psdo_0000022 -->

    <owl:Class rdf:about="http://purl.obolibrary.org/obo/psdo#psdo_0000022">
        <rdfs:subClassOf rdf:resource="http://purl.obolibrary.org/obo/psdo#psdo_0000020"/>
        <rdfs:label xml:lang="en">continuous scale types</rdfs:label>
    </owl:Class>
    


    <!-- http://purl.obolibrary.org/obo/psdo#psdo_0000023 -->

    <owl:Class rdf:about="http://purl.obolibrary.org/obo/psdo#psdo_0000023">
        <rdfs:subClassOf rdf:resource="http://purl.obolibrary.org/obo/psdo#psdo_0000022"/>
        <obo:IAO_0000115>a continuous scale with three formal properties that (1) the instances can be distinguished from each another and (2) that one instance on a scale can be judged greater than, less than, or equal to another instance on the same scale and that (3) the magnitude of an instance represented by a unit on the scale is the same regardless of where on the scale the unit falls</obo:IAO_0000115>
        <obo:IAO_0000119>1. Zhang J. A representational analysis of relational information displays. International Journal of Human-Computer Studies. 1996 Jul 1;45(1):59–74.</obo:IAO_0000119>
        <rdfs:label xml:lang="en">interval scale</rdfs:label>
    </owl:Class>
    


    <!-- http://purl.obolibrary.org/obo/psdo#psdo_0000024 -->

    <owl:Class rdf:about="http://purl.obolibrary.org/obo/psdo#psdo_0000024">
        <rdfs:subClassOf rdf:resource="http://purl.obolibrary.org/obo/psdo#psdo_0000022"/>
        <obo:IAO_0000115>a continuous scale with four formal properties that (1) the instances can be distinguished from each another and (2) that one instance on a scale can be judged greater than, less than, or equal to another instance on the same scale, that (3) the magnitude of an instance represented by a unit on the scale is the same regardless of where on the scale the unit falls and (4) an absolute zero value can indicate that nothing at all of the property being represented exists</obo:IAO_0000115>
        <obo:IAO_0000119>1. Zhang J. A representational analysis of relational information displays. International Journal of Human-Computer Studies. 1996 Jul 1;45(1):59–74.</obo:IAO_0000119>
        <rdfs:label xml:lang="en">ratio scale</rdfs:label>
    </owl:Class>
    


    <!-- http://purl.obolibrary.org/obo/psdo#psdo_0000025 -->

    <owl:Class rdf:about="http://purl.obolibrary.org/obo/psdo#psdo_0000025">
        <rdfs:subClassOf rdf:resource="http://purl.obolibrary.org/obo/psdo#psdo_0000021"/>
        <obo:IAO_0000115>a dicrete scale with two formal properties that (1) the instances can be distinguished from each another and (2) that one instance on a scale can be judged greater than, less than, or equal to another instance on the same scale</obo:IAO_0000115>
        <obo:IAO_0000119>1. Zhang J. A representational analysis of relational information displays. International Journal of Human-Computer Studies. 1996 Jul 1;45(1):59–74.</obo:IAO_0000119>
        <rdfs:label xml:lang="en">oridinal scale</rdfs:label>
    </owl:Class>
    


    <!-- http://purl.obolibrary.org/obo/psdo#psdo_0000026 -->

    <owl:Class rdf:about="http://purl.obolibrary.org/obo/psdo#psdo_0000026">
        <rdfs:subClassOf rdf:resource="http://purl.obolibrary.org/obo/psdo#psdo_0000021"/>
        <obo:IAO_0000115>a dicrete scale with one  formal property that (1) the instances can be distinguished from each another</obo:IAO_0000115>
        <obo:IAO_0000119>1. Zhang J. A representational analysis of relational information displays. International Journal of Human-Computer Studies. 1996 Jul 1;45(1):59–74.</obo:IAO_0000119>
        <rdfs:label xml:lang="en">nominal scale</rdfs:label>
    </owl:Class>
    


    <!-- http://purl.obolibrary.org/obo/psdo#psdo_0000027 -->

    <owl:Class rdf:about="http://purl.obolibrary.org/obo/psdo#psdo_0000027">
        <rdfs:label xml:lang="en">time series</rdfs:label>
    </owl:Class>
    


    <!-- http://purl.obolibrary.org/obo/psdo#psdo_0000028 -->

    <owl:Class rdf:about="http://purl.obolibrary.org/obo/psdo#psdo_0000028">
        <obo:IAO_0000115>the general movement over time of a detectable change in performance</obo:IAO_0000115>
        <rdfs:label xml:lang="en">performance trend</rdfs:label>
    </owl:Class>
    


    <!-- http://purl.obolibrary.org/obo/psdo#psdo_0000029 -->

    <owl:Class rdf:about="http://purl.obolibrary.org/obo/psdo#psdo_0000029">
        <obo:IAO_0000115>A numerical difference between the performance data of a performer for a performance measure and some comparator.</obo:IAO_0000115>
        <rdfs:label xml:lang="en">gap</rdfs:label>
    </owl:Class>
    


    <!-- http://purl.obolibrary.org/obo/psdo#psdo_0000030 -->

    <owl:Class rdf:about="http://purl.obolibrary.org/obo/psdo#psdo_0000030">
        <obo:IAO_0000115>The smallest quantity of data from which meaningful inferences and/or evaluations can be made. (i.e. threshold)</obo:IAO_0000115>
        <rdfs:label xml:lang="en">minimally sufficient data</rdfs:label>
    </owl:Class>
    


    <!-- http://purl.obolibrary.org/obo/psdo#psdo_0000031 -->

    <owl:Class rdf:about="http://purl.obolibrary.org/obo/psdo#psdo_0000031">
        <rdfs:subClassOf rdf:resource="http://purl.obolibrary.org/obo/IAO_0000088"/>
        <obo:IAO_0000115>a report that contains information about at least one performer and at least one performance measure</obo:IAO_0000115>
        <rdfs:label xml:lang="en">performance report</rdfs:label>
    </owl:Class>
    


    <!-- http://purl.obolibrary.org/obo/psdo#psdo_0000032 -->

    <owl:Class rdf:about="http://purl.obolibrary.org/obo/psdo#psdo_0000032">
        <rdfs:subClassOf rdf:resource="http://purl.obolibrary.org/obo/psdo#psdo_0000005"/>
        <obo:IAO_0000115>the number of &apos;n&apos; mutually perpendicular directions of motion that are possible in the time dimension</obo:IAO_0000115>
        <rdfs:label xml:lang="en">time dimension cardinality</rdfs:label>
    </owl:Class>
    


    <!-- http://purl.obolibrary.org/obo/psdo#psdo_0000033 -->

    <owl:Class rdf:about="http://purl.obolibrary.org/obo/psdo#psdo_0000033">
        <rdfs:subClassOf rdf:resource="http://purl.obolibrary.org/obo/psdo#psdo_0000005"/>
        <obo:IAO_0000115>the number of &apos;n&apos; mutually perpendicular directions of motion that are possible in the performer dimension</obo:IAO_0000115>
        <obo:IAO_0000116>Informally, this can be viewed as the number of different dimensions representing performers</obo:IAO_0000116>
        <rdfs:label xml:lang="en">performer dimension cardinality</rdfs:label>
    </owl:Class>
    


    <!-- http://purl.obolibrary.org/obo/psdo#psdo_0000034 -->

    <owl:Class rdf:about="http://purl.obolibrary.org/obo/psdo#psdo_0000034">
        <rdfs:subClassOf rdf:resource="http://purl.obolibrary.org/obo/psdo#psdo_0000005"/>
        <obo:IAO_0000115>the number of &apos;n&apos; mutually perpendicular directions of motion that are possible in the performance measure dimension</obo:IAO_0000115>
        <obo:IAO_0000116>Informally, this can be viewed as the total number of different measures, measurements, or expressions of measured behavior</obo:IAO_0000116>
        <rdfs:label xml:lang="en">performance measure dimension cardinality</rdfs:label>
    </owl:Class>
    


    <!-- http://purl.obolibrary.org/obo/psdo#psdo_0000035 -->

    <owl:Class rdf:about="http://purl.obolibrary.org/obo/psdo#psdo_0000035">
        <rdfs:subClassOf rdf:resource="http://purl.obolibrary.org/obo/psdo#psdo_0000006"/>
        <obo:IAO_0000115>a vector that represents the measurements, aggragates, and/or calculations that represent a measured behavior</obo:IAO_0000115>
        <rdfs:label xml:lang="en">performance measure dimension</rdfs:label>
    </owl:Class>
    


    <!-- http://purl.obolibrary.org/obo/psdo#psdo_0000036 -->

    <owl:Class rdf:about="http://purl.obolibrary.org/obo/psdo#psdo_0000036">
        <rdfs:subClassOf rdf:resource="http://purl.obolibrary.org/obo/psdo#psdo_0000006"/>
        <obo:IAO_0000115>a vector that represents time</obo:IAO_0000115>
        <rdfs:label xml:lang="en">time dimension</rdfs:label>
    </owl:Class>
    


    <!-- http://purl.obolibrary.org/obo/psdo#psdo_0000037 -->

    <owl:Class rdf:about="http://purl.obolibrary.org/obo/psdo#psdo_0000037">
        <rdfs:subClassOf rdf:resource="http://purl.obolibrary.org/obo/psdo#psdo_0000006"/>
        <obo:IAO_0000115>does this dimension really exist, or can the other three dimensions fully epxress the information we need them to?</obo:IAO_0000115>
        <rdfs:label xml:lang="en">performance data dimension</rdfs:label>
    </owl:Class>
    


    <!-- http://purl.obolibrary.org/obo/psdo#psdo_0000038 -->

    <owl:Class rdf:about="http://purl.obolibrary.org/obo/psdo#psdo_0000038">
        <rdfs:subClassOf rdf:resource="http://purl.obolibrary.org/obo/psdo#psdo_0000005"/>
        <obo:IAO_0000115>the number of &apos;n&apos; mutually perpendicular directions of motion that are possible in a performance data dimension</obo:IAO_0000115>
        <rdfs:label xml:lang="en">performance data dimension cardinality</rdfs:label>
    </owl:Class>
</rdf:RDF>



<!-- Generated by the OWL API (version 4.2.8.20170104-2310) https://github.com/owlcs/owlapi -->

